Phi_Semantics/PhiSem_Agg_Void.thy
@@ -5,5 +5,14 @@ begin
 debt_axiomatization
     valid_idx_step_void[eval_aggregate_path] : \<open>valid_idx_step void i \<longleftrightarrow> False\<close>
 
+lemma valid_index_void[iff]:
+  \<open>valid_index void path \<longleftrightarrow> path = []\<close>
+  by (induct path; simp add: valid_idx_step_void)
+
+lemma [\<phi>reason 1000]:
+  \<open> \<c>\<o>\<n>\<d>\<i>\<t>\<i>\<o>\<n> path = []
+\<Longrightarrow> valid_index void path\<close>
+  unfolding Premise_def
+  by simp
 
 end
