Phi_Semantics/PhiSem_Mem_Ptr_Machine_Int.thy
@@ -4,26 +4,5 @@ begin
 
 subsection \<open>Instruction\<close>
 
-proc op_get_element_pointer_numidx:
-  requires \<open>\<c>\<o>\<n>\<d>\<i>\<t>\<i>\<o>\<n>[eval_aggregate_path] valid_idx_step TY AG_IDX(#i)\<close>
-       and \<open> \<s>\<i>\<m>\<p>\<l>\<i>\<f>\<y>[eval_aggregate_path] TY' : idx_step_type AG_IDX(#i) TY\<close>
-  input  \<open>addr \<Ztypecolon> \<v>\<a>\<l> Ptr TY\<heavy_comma> i \<Ztypecolon> \<v>\<a>\<l> \<nat>('b)\<close>
-  output \<open>addr \<tribullet>\<^sub>a LOGIC_IDX(AgIdx_N i) \<Ztypecolon> \<v>\<a>\<l> Ptr TY'\<close>
-\<medium_left_bracket>
-  $addr semantic_local_value pointer
-  $i semantic_local_value \<open>int('b)\<close>
-  semantic_return \<open>
-     V_pointer.mk (logaddr_to_raw (rawaddr_to_log TY (V_pointer.dest (\<phi>arg.dest \<a>\<r>\<g>1)) \<tribullet>\<^sub>a LOGIC_IDX(AgIdx_N (snd (V_int.dest (\<phi>arg.dest \<a>\<r>\<g>2))))))
-         \<in> (addr \<tribullet>\<^sub>a LOGIC_IDX(AgIdx_N i) \<Ztypecolon> Ptr TY')\<close>
-  certified by ((insert useful, simp add: \<phi>expns;
-        cases \<open>phantom_mem_semantic_type (logaddr_type addr)\<close>;
-        cases \<open>addr = 0\<close>;
-        simp add: logaddr_to_raw_phantom_mem_type),
-        (insert valid_idx_step_void, blast)[1],
-        (smt logaddr_to_raw_phantom_mem_type rawaddr_to_log_def someI_ex),
-        (insert valid_idx_step_void,blast)[1],
-        force)
-\<medium_right_bracket> .
-
 
 end
